src/lib/data/Kuiper.Tensor.Layout.Alg.fst
@@ -52,7 +52,7 @@ instance cunit : auto_cinj lunit = {
   ff = (fun _ -> 0sz);
 }
 
-// #restart-solver // work around crash
+#push-options "--z3rlimit 40"
 inline_for_extraction noextract
 let c_major_on_f
   (#n: erased nat)
@@ -61,21 +61,27 @@ let c_major_on_f
   (#d : idesc n)
   {| cs : csizeof d |}
   (#sub : layout_f_for d)
+  (#_ : squash (SZ.fits (k * sizeof d)))
   (c_sub : auto_cinj sub)
   (idx:conc (insert_i i k d))
   : r : szlt (sizeof (insert_i i k d)) { SZ.v r == major_on_f i k sub (up idx) }
   = // let maj, min = c_bring_forward_ff i (insert_i i k d) idx in
     // ^ Still unclear why something like this does not extract, but the below does.
     match c_bring_forward_ff (SZ.v i) (insert_i i k d) idx with maj, min ->
+    assert (maj < (insert_i i k d) @! i);
+    assert ((insert_i i k d) @! i == reveal k);
+    assert (maj < k);
     match c_sub with { ff } ->
     let sub_i : szlt (sizeof d) = ff min in
     lemma_c_bring_forward_ff_ok i (insert_i i k d) idx;
     bring_forward_commute2 i (insert_i i k d) maj min;
-    assume (SZ.fits (maj * cs.v));
+    assert (maj * cs.v <= (k-1) * sizeof d);
     let offset : SZ.t = maj *^ cs.v in
-    assume (SZ.fits (offset + sub_i));
+    assert (sub_i < sizeof d);
+    assert (maj * cs.v + sub_i < k * sizeof d);
     let r = offset +^ sub_i in
     r
+#pop-options
 
 inline_for_extraction noextract
 instance c_major_on
@@ -85,14 +91,15 @@ instance c_major_on
   (#d : idesc n)
   {| cs : csizeof d |}
   (#sub : layout_f_for d)
+  (#_ : squash (SZ.fits (k * sizeof d)))
   (c_sub : auto_cinj sub)
   : auto_cinj (major_on i k sub) =
   { ff = c_major_on_f i k c_sub; }
 
 inline_for_extraction noextract
 instance c_pack (#n : erased nat) (#d: idesc n)
-  {| culen : csizeof d |}
   (#f : layout_f_for d) (c_f : auto_cinj f)
+  (#_ : squash (SZ.fits (sizeof d)))
   (#_ : squash (all_fit d))
   : ctlayout (pack f) =
   {
